---
layout: post
title: "Fundamentals of Nanoelectronics: Lecture 1.4"
hide: true
---

This is the [fourth lecture](https://www.youtube.com/watch?v=_MlI1E6z9e4)

In this lecture, we derive an expression for the overall conductance in terms of the Fermi Function
and G(E) which is the conductance depending on the energy.

We start with the current formula derived in the previous lecture:

$I = \frac{1}{q} \int_{-\infty}^{\infty} G(E) (f_1(E) - f_2(E)) dE$

Here $f_1(E)$ and $f_2(E)$ are respectively,
$f_1(E) = f(E,\mu _1) = \frac{1}{1+ \e ^ \frac{E-\mu _1}{kT}}$

$f_2(E) = f(E,\mu _2) = \frac{1}{1+ \e ^ \frac{E-\mu _2}{kT}}$

Taking a short diversion, in the Fermi Function:
$f(E) = frac{1}{1+ \e ^ \frac{E-\mu}{kT}}$

If we replace $\frac{E-\mu}{kT}$ with $x$, we have:
$f(x) = \frac {1}{1+\e ^ x}$

So, the partial derivative of $f(E)$ with respect to E is:
$\frac{\partial f}{\partial E} = \frac{\partial f}{\partial x} * \frac{\partial x}{\partial E}$

Similarly, the partial derivative of $f(E)$ with respect to $\mu$ is:
$\frac{\partial f}{\partial \mu} = \frac{\partial f}{\partial x} * \frac{\partial x}{\partial \mu}$

From, $x = \frac {E-\mu} {kT}$:

$\frac{\partial x}{\partial E} = \frac {1}{kT}$, and
$\frac{\partial x}{\partial \mu}= -\frac{1}{kT}$

From the above two, we have the relation
$\frac{\partial x}{\partial E} = - $\frac{\partial x}{\partial \mu}$

When $\mu _1$ and $\mu _2$ are close values, ie. for small V, from the Taylor series, we have:

$f(E, \mu _1) - f(E, \mu _2) \approx (\frac{\partial f}{\partial \mu})_\mu _0 (\mu _1 - \mu _2)$

Reformulating this in terms of partial derivative of E,

$RHS = (-\frac{\partial f}{\partial \E})_\mu _0 (\mu _1 - \mu _2)$

Therefore,
$I =  \frac{1}{q} \int_{-\infty}^{\infty} G(E) (-\frac{\partial f}{\partial \E})_\mu _0 (\mu _1 - \mu _2) dE$
$\mu _1 - \mu _2 = qV$

So,
$I/V = \int_{-\infty}^{\infty} G(E) (-\frac{\partial f}{\partial \E})_\mu _0 dE$

The above formula indicates that the measured conductance is an average of the conductance function. 